Update sources (PLF: v6.0, VFA: v1.5, QC: v1.2 and VC: v1.1.0) and add sources (SLF: v1.0).
* PLF: v5.8   -> v6.0
* VFA: v1.4   -> v1.5
* QC:  v1.1   -> v1.2
* VC:  v0.9.7 -> v1.1.0
* SLF:        -> v1.0 (new)

src/plf/References.v
@@ -29,13 +29,16 @@
     the refinement we need to make to the statement of the type
     preservation theorem. *)
 
-Set Warnings "-notation-overridden,-parsing".
+Set Warnings "-notation-overridden,-parsing,-deprecated-hint-without-locality".
 From Coq Require Import Strings.String.
+From Coq Require Import Init.Nat.
 From Coq Require Import Arith.Arith.
+From Coq Require Import Arith.PeanoNat.
 From Coq Require Import Lia.
 From PLF Require Import Maps.
 From PLF Require Import Smallstep.
 From Coq Require Import Lists.List.
+Import Nat.
 
 (* ################################################################# *)
 (** * Definitions *)
@@ -170,7 +173,7 @@ Notation "'Unit'" :=
   (Ty_Unit) (in custom stlc at level 0).
 Notation "'unit'" := tm_unit (in custom stlc at level 0).
 
-Notation "'Natural'" := Ty_Nat (in custom stlc at level 0).
+Notation "'Nat'" := Ty_Nat (in custom stlc at level 0).
 Notation "'succ' x" := (tm_succ x) (in custom stlc at level 0,
                                      x custom stlc at level 0).
 Notation "'pred' x" := (tm_pred x) (in custom stlc at level 0,
@@ -436,7 +439,7 @@ Notation "t1 ; t2" := (tseq t1 t2) (in custom stlc at level 3).
       r2  // yields 1, not 2!
 *)
 
-(** **** Exercise: 1 star, standard, optional (store_draw) 
+(** **** Exercise: 1 star, standard, optional (store_draw)
 
     Draw (on paper) the contents of the store at the point in
     execution where the first two [let]s have finished and the third
@@ -453,15 +456,15 @@ Notation "t1 ; t2" := (tseq t1 t2) (in custom stlc at level 3).
     we've defined above allow us to create references to values of any
     type, including functions.  For example, we can use references to
     functions to give an (inefficient) implementation of arrays
-    of numbers, as follows.  Write [NaturalArray] for the type
-    [Ref (Natural->Natural)].
+    of numbers, as follows.  Write [NatArray] for the type
+    [Ref (Nat->Nat)].
 
     Recall the [equal] function from the [MoreStlc] chapter:
 
       equal =
         fix
-          (\eq:Natural->Natural->Bool.
-             \m:Natural. \n:Natural.
+          (\eq:Nat->Nat->Bool.
+             \m:Nat. \n:Nat.
                if m=0 then iszero n
                else if n=0 then false
                else eq (pred m) (pred n))
@@ -469,12 +472,12 @@ Notation "t1 ; t2" := (tseq t1 t2) (in custom stlc at level 3).
     To build a new array, we allocate a reference cell and fill
     it with a function that, when given an index, always returns [0].
 
-      newarray = \_:Unit. ref (\n:Natural.0)
+      newarray = \_:Unit. ref (\n:Nat.0)
 
     To look up an element of an array, we simply apply
     the function to the desired index.
 
-      lookup = \a:NaturalArray. \n:Natural. (!a) n
+      lookup = \a:NatArray. \n:Nat. (!a) n
 
     The interesting part of the encoding is the [update] function.  It
     takes an array, an index, and a new value to be stored at that index, and
@@ -483,20 +486,20 @@ Notation "t1 ; t2" := (tseq t1 t2) (in custom stlc at level 3).
     value that was given to [update], while on all other indices it passes the
     lookup to the function that was previously stored in the reference.
 
-      update = \a:NaturalArray. \m:Natural. \v:Natural.
+      update = \a:NatArray. \m:Nat. \v:Nat.
                    let oldf = !a in
-                   a := (\n:Natural. if equal m n then v else oldf n);
+                   a := (\n:Nat. if equal m n then v else oldf n);
 
     References to values containing other references can also be very
     useful, allowing us to define data structures such as mutable
     lists and trees. *)
 
-(** **** Exercise: 2 stars, standard, especially useful (compact_update) 
+(** **** Exercise: 2 stars, standard, especially useful (compact_update)
 
     If we defined [update] more compactly like this
 
-      update = \a:NaturalArray. \m:Natural. \v:Natural.
-                  a := (\n:Natural. if equal m n then v else (!a) n)
+      update = \a:NatArray. \m:Nat. \v:Nat.
+                  a := (\n:Nat. if equal m n then v else (!a) n)
 
 would it behave the same? *)
 
@@ -550,10 +553,10 @@ Definition manual_grade_for_compact_update : option (nat*string) := None.
     a number, save a reference to it in some data structure, use it
     for a while, then deallocate it and allocate a new cell holding a
     boolean, possibly reusing the same storage.  Now we can have two
-    names for the same storage cell -- one with type [Ref Natural] and the
+    names for the same storage cell -- one with type [Ref Nat] and the
     other with type [Ref Bool]. *)
 
-(** **** Exercise: 2 stars, standard (type_safety_violation) 
+(** **** Exercise: 2 stars, standard (type_safety_violation)
 
     Show how this can lead to a violation of type safety. *)
 
@@ -848,17 +851,17 @@ Inductive step : tm * store -> tm * store -> Prop :=
          t2 / st --> t2' / st' ->
          <{ v1 t2 }> / st --> <{ v1 t2' }> / st'
   (* numbers *)
-  | ST_SuccNatural : forall (n : nat) st,
+  | ST_SuccNat : forall (n : nat) st,
          <{ succ n }> / st --> tm_const (S n) / st
   | ST_Succ : forall t1 t1' st st',
          t1 / st --> t1' / st' ->
          <{ succ t1 }> / st --> <{ succ t1' }> / st'
-  | ST_PredNatural : forall (n : nat) st,
+  | ST_PredNat : forall (n : nat) st,
          <{ pred n }> / st --> tm_const (n - 1) / st
   | ST_Pred : forall t1 t1' st st',
          t1 / st --> t1' / st' ->
          <{ pred t1 }> / st --> <{ pred t1' }> / st'
-  | ST_MultNaturals : forall (n1 n2 : nat) st,
+  | ST_MultNats : forall (n1 n2 : nat) st,
       <{ n1 * n2 }> / st -->  tm_const (n1 * n2) / st
   | ST_Mult1 : forall t1 t2 t1' st st',
          t1 / st --> t1' / st' ->
@@ -990,10 +993,10 @@ Definition context := partial_map ty.
     there is no finite typing derivation for the location [0] with respect
     to this store:
 
-   [\x:Natural. (!(loc 1)) x, \x:Natural. (!(loc 0)) x]
+   [\x:Nat. (!(loc 1)) x, \x:Nat. (!(loc 0)) x]
 *)
 
-(** **** Exercise: 2 stars, standard (cyclic_store) 
+(** **** Exercise: 2 stars, standard (cyclic_store)
 
     Can you find a term whose reduction will create this particular
     cyclic store? *)
@@ -1092,20 +1095,20 @@ Inductive has_type (ST : store_ty) : context -> tm -> ty -> Prop :=
       Gamma ; ST |- t1 \in (T2 -> T1) ->
       Gamma ; ST |- t2 \in T2 ->
       Gamma ; ST |- t1 t2 \in T1
-  | T_Natural : forall Gamma (n : nat),
-      Gamma ; ST |- n \in Natural
+  | T_Nat : forall Gamma (n : nat),
+      Gamma ; ST |- n \in Nat
   | T_Succ : forall Gamma t1,
-      Gamma ; ST |- t1 \in Natural ->
-      Gamma ; ST |- succ t1 \in Natural
+      Gamma ; ST |- t1 \in Nat ->
+      Gamma ; ST |- succ t1 \in Nat
   | T_Pred : forall Gamma t1,
-      Gamma ; ST |- t1 \in Natural ->
-      Gamma ; ST |- pred t1 \in Natural
+      Gamma ; ST |- t1 \in Nat ->
+      Gamma ; ST |- pred t1 \in Nat
   | T_Mult : forall Gamma t1 t2,
-      Gamma ; ST |- t1 \in Natural ->
-      Gamma ; ST |- t2 \in Natural ->
-      Gamma ; ST |- t1 * t2 \in Natural
+      Gamma ; ST |- t1 \in Nat ->
+      Gamma ; ST |- t2 \in Nat ->
+      Gamma ; ST |- t1 * t2 \in Nat
   | T_If0 : forall Gamma t1 t2 t3 T0,
-      Gamma ; ST |- t1 \in Natural ->
+      Gamma ; ST |- t1 \in Nat ->
       Gamma ; ST |- t2 \in T0 ->
       Gamma ; ST |- t3 \in T0 ->
       Gamma ; ST |- if0 t1 then t2 else t3 \in T0
@@ -1204,7 +1207,7 @@ Definition store_well_typed (ST:store_ty) (st:store) :=
     typing to the typing relation.  This allows us to type circular
     stores like the one we saw above. *)
 
-(** **** Exercise: 2 stars, standard (store_not_unique) 
+(** **** Exercise: 2 stars, standard (store_not_unique)
 
     Can you find a store [st], and two
     different store typings [ST1] and [ST2] such that both
@@ -1353,7 +1356,7 @@ Lemma weakening : forall Gamma Gamma' ST t T,
      Gamma  ; ST |- t \in T  ->
      Gamma' ; ST |- t \in T.
 Proof.
-  intros Gamma Gamma' ST t T H Ht. 
+  intros Gamma Gamma' ST t T H Ht.
   generalize dependent Gamma'.
   induction Ht; eauto using inclusion_update.
 Qed.
@@ -1374,7 +1377,7 @@ Lemma substitution_preserves_typing : forall Gamma ST x U t v T,
 Proof.
   intros Gamma ST x U t v T Ht Hv.
   generalize dependent Gamma. generalize dependent T.
-  induction t; intros T Gamma H; 
+  induction t; intros T Gamma H;
   (* in each case, we'll want to get at the derivation of H *)
     inversion H; clear H; subst; simpl; eauto.
   - (* var *)
@@ -1386,7 +1389,7 @@ Proof.
     + (* x<>y *)
       apply T_Var. rewrite update_neq in H2; auto.
   - (* abs *)
-    rename s into y, t into T.
+    rename s into y.
     destruct (eqb_stringP x y); subst; apply T_Abs.
     + (* x=y *)
       rewrite update_shadow in H5. assumption.
@@ -1415,10 +1418,10 @@ Proof with auto.
   intros l' Hl'.
   destruct (l' =? l) eqn: Heqll'.
   - (* l' = l *)
-    apply Nat.eqb_eq in Heqll'; subst.
+    apply eqb_eq in Heqll'; subst.
     rewrite lookup_replace_eq...
   - (* l' <> l *)
-    apply Nat.eqb_neq in Heqll'.
+    apply eqb_neq in Heqll'.
     rewrite lookup_replace_neq...
     rewrite length_replace in Hl'.
     apply H0...
@@ -1462,8 +1465,8 @@ Proof with auto.
   intros.
   unfold store_well_typed in *.
   destruct H as [Hlen Hmatch].
-  rewrite app_length, plus_comm. simpl.
-  rewrite app_length, plus_comm. simpl.
+  rewrite app_length, add_comm. simpl.
+  rewrite app_length, add_comm. simpl.
   split...
   - (* types match. *)
     intros l Hl.
@@ -1563,7 +1566,7 @@ Proof with eauto using store_weakening, extends_refl.
     { replace <{ Ref T1 }>
         with <{ Ref {store_Tlookup (length st) (ST ++ T1::nil)} }>.
       { apply T_Loc.
-        rewrite <- H. rewrite app_length, plus_comm. simpl. lia. }
+        rewrite <- H. rewrite app_length, add_comm. simpl. lia. }
       unfold store_Tlookup. rewrite <- H. rewrite nth_eq_last.
       reflexivity. }
     apply store_well_typed_app; assumption.
@@ -1597,7 +1600,7 @@ Proof with eauto using store_weakening, extends_refl.
     exists ST'...
 Qed.
 
-(** **** Exercise: 3 stars, standard (preservation_informal) 
+(** **** Exercise: 3 stars, standard (preservation_informal)
 
     Write a careful informal proof of the preservation theorem,
     concentrating on the [T_App], [T_Deref], [T_Assign], and [T_Ref]
@@ -1764,7 +1767,7 @@ Definition loop :=
 
 Lemma loop_typeable : exists T, empty; nil |- loop \in T.
 Proof with eauto.
-  eexists. unfold loop. unfold loop_fun. 
+  eexists. unfold loop. unfold loop_fun.
   eapply T_App...
   eapply T_Abs...
   eapply T_App...
@@ -1838,7 +1841,7 @@ Proof with eauto.
   eapply sc_one. compute. apply ST_AppAbs...
 Qed.
 
-(** **** Exercise: 4 stars, standard (factorial_ref) 
+(** **** Exercise: 4 stars, standard (factorial_ref)
 
     Use the above ideas to implement a factorial function in STLC with
     references.  (There is no need to prove formally that it really
@@ -1849,7 +1852,7 @@ Qed.
 Definition factorial : tm
   (* REPLACE THIS LINE WITH ":= _your_definition_ ." *). Admitted.
 
-Lemma factorial_type : empty; nil |- factorial \in (Natural -> Natural).
+Lemma factorial_type : empty; nil |- factorial \in (Nat -> Nat).
 Proof with eauto.
   (* FILL IN HERE *) Admitted.
 
@@ -1869,7 +1872,7 @@ Qed.
 (* ################################################################# *)
 (** * Additional Exercises *)
 
-(** **** Exercise: 5 stars, standard, optional (garabage_collector) 
+(** **** Exercise: 5 stars, standard, optional (garabage_collector)
 
     Challenge problem: modify our formalization to include an account
     of garbage collection, and prove that it satisfies whatever nice
@@ -1880,4 +1883,4 @@ Qed.
 End RefsAndNontermination.
 End STLCRef.
 
-(* 2020-09-09 21:08 *)
+(* 2021-05-26 09:57 *)
