src/qc/QuickChickTool.v
@@ -501,4 +501,4 @@ Definition compiles_correctly (e : exp) := (execute [] (compile e)) = [eval e]?.
     in [QuickChickInterface].
 *)
 
-(* 2020-10-14 10:23 *)
+(* 2021-05-26 10:04 *)
