src/vfa/MergeTest.v
@@ -171,4 +171,6 @@ idtac "---------- mergesort_perm ---------".
 Print Assumptions mergesort_perm.
 Abort.
 
-(* 2020-08-07 17:08 *)
+(* 2021-05-26 10:00 *)
+
+(* 2021-05-26 10:00 *)
