src/vfa/MultisetTest.v
@@ -288,4 +288,6 @@ idtac "---------- contents_perm ---------".
 Print Assumptions contents_perm.
 Abort.
 
-(* 2020-08-07 17:08 *)
+(* 2021-05-26 10:00 *)
+
+(* 2021-05-26 10:00 *)
