src/vfa/SortTest.v
@@ -175,4 +175,6 @@ idtac "---------- sorted'_sorted ---------".
 Print Assumptions sorted'_sorted.
 Abort.
 
-(* 2020-08-07 17:08 *)
+(* 2021-05-26 10:00 *)
+
+(* 2021-05-26 10:00 *)
